further speedups

src/v3/circuit.lean
@@ -11,7 +11,6 @@ inductive circuit (α : Type u) : Type u
 | or : circuit → circuit → circuit
 | not : circuit → circuit
 | xor : circuit → circuit → circuit
-| imp : circuit → circuit → circuit
 
 namespace circuit
 variables {α : Type u} {β : Type v}
@@ -24,7 +23,6 @@ def reppr [has_repr α] : (circuit α) → string
 | (or x y) := "(" ++ reppr x ++ " ∨ " ++ reppr y ++ ")"
 | (not x) := "¬" ++ reppr x
 | (xor x y) := "(" ++ reppr x ++ " ⊕ " ++ reppr y ++ ")"
-| (imp x y) := "(" ++ reppr x ++ " → " ++ reppr y ++ ")"
 
 instance [has_repr α] : has_repr (circuit α) := ⟨reppr⟩
 
@@ -36,7 +34,6 @@ def vars [decidable_eq α] : circuit α → list α
 | (or c₁ c₂) := (vars c₁ ++ vars c₂).dedup
 | (not c) := vars c
 | (xor c₁ c₂) := (vars c₁ ++ vars c₂).dedup
-| (imp c₁ c₂) := (vars c₁ ++ vars c₂).dedup
 
 @[simp] def eval : circuit α → (α → bool) → bool
 | true _ := tt
@@ -46,7 +43,6 @@ def vars [decidable_eq α] : circuit α → list α
 | (or c₁ c₂) f := (eval c₁ f) || (eval c₂ f)
 | (not c) f := bnot (eval c f)
 | (xor c₁ c₂) f := bxor (eval c₁ f) (eval c₂ f)
-| (imp c₁ c₂) f := bnot (eval c₁ f) || (eval c₂ f)
 
 @[simp] def evalv [decidable_eq α] : Π (c : circuit α), (Π a ∈ vars c, bool) → bool
 | true _ := tt
@@ -59,8 +55,6 @@ def vars [decidable_eq α] : circuit α → list α
 | (not c) f := bnot (evalv c (λ i hi, f i (by simp [hi, vars])))
 | (xor c₁ c₂) f := bxor (evalv c₁ (λ i hi, f i (by simp [hi, vars])))
   (evalv c₂ (λ i hi, f i (by simp [hi, vars])))
-| (imp c₁ c₂) f := bnot (evalv c₁ (λ i hi, f i (by simp [hi, vars]))) ||
-  (evalv c₂ (λ i hi, f i (by simp [hi, vars])))
 
 lemma eval_eq_evalv [decidable_eq α] : ∀ (c : circuit α) (f : α → bool),
   eval c f = evalv c (λ x _, f x)
@@ -71,7 +65,6 @@ lemma eval_eq_evalv [decidable_eq α] : ∀ (c : circuit α) (f : α → bool),
 | (or c₁ c₂) f := by rw [eval, evalv, eval_eq_evalv, eval_eq_evalv]
 | (not c) f := by rw [eval, evalv, eval_eq_evalv]
 | (xor c₁ c₂) f := by rw [eval, evalv, eval_eq_evalv, eval_eq_evalv]
-| (imp c₁ c₂) f := by rw [eval, evalv, eval_eq_evalv, eval_eq_evalv]
 
 @[simp] def of_bool : bool → circuit α
 | tt := true
@@ -85,12 +78,25 @@ instance : preorder (circuit α) :=
   le_refl := λ c f h, h,
   le_trans := λ c₁ c₂ c₃ h₁₂ h₂₃ f h₁, h₂₃ f (h₁₂ f h₁) }
 
-instance [decidable_eq α] :
-  decidable_rel ((≤) : circuit α → circuit α → Prop) :=
-λ c₁ c₂, decidable_of_iff (∀ (x : Π (i : α), (i ∈ (c₁.vars ++ c₂.vars).dedup) → bool),
-  x ∈ (c₁.vars ++ c₂.vars).dedup.pi (λ _, [tt, ff]) →
-  c₁.evalv (λ i hi, x i (by simp [hi])) → c₂.evalv (λ i hi, x i (by simp [hi])))
-   sorry
+lemma le_def : ∀ (c₁ c₂ : circuit α), c₁ ≤ c₂ ↔ ∀ f, eval c₁ f → eval c₂ f :=
+λ _ _, iff.rfl
+
+lemma exists_eval_iff_exists_evalv [decidable_eq α] (c : circuit α) :
+  (∃ x, eval c x) ↔ ∃ x, evalv c x :=
+begin
+  split,
+  { rintro ⟨x, hx⟩,
+    use λ a _, x a,
+    rw [eval_eq_evalv] at hx,
+    exact hx },
+  { rintro ⟨x, hx⟩,
+    refine ⟨λ a, dite (a ∈ c.vars) (x a) (λ _, ff), _⟩,
+    convert hx,
+    rw [eval_eq_evalv],
+    congr' 1,
+    ext i hi,
+    simp [hi] }
+end
 
 def simplify_and : circuit α → circuit α → circuit α
 | true c := c
@@ -150,20 +156,6 @@ begin
   cases c₁; cases c₂; simp [*, circuit.simplify_xor, eval, bnot_bxor] at *,
 end
 
-def simplify_imp : circuit α → circuit α → circuit α
-| false _ := true
-| _ true := true
-| true c := c
-| c false := not c
-| c₁ c₂ := imp c₁ c₂
-
-@[simp] lemma eval_simplify_imp : ∀ (c₁ c₂ : circuit α) (f : α → bool),
-  eval (simplify_imp c₁ c₂) f = bnot (eval c₁ f) || (eval c₂ f) :=
-begin
-  intros c₁ c₂ f,
-  cases c₁; cases c₂; simp [*, circuit.simplify_imp, eval] at *
-end
-
 def map : Π (c : circuit α) (f : α → β), circuit β
 | true _ := true
 | false _ := false
@@ -172,7 +164,6 @@ def map : Π (c : circuit α) (f : α → β), circuit β
 | (or c₁ c₂) f := simplify_or (map c₁ f) (map c₂ f)
 | (not c) f := simplify_not (map c f)
 | (xor c₁ c₂) f := simplify_xor (map c₁ f) (map c₂ f)
-| (imp c₁ c₂) f := simplify_imp (map c₁ f) (map c₂ f)
 
 lemma eval_map {c : circuit α} {f : α → β} {g : β → bool} :
   eval (map c f) g = eval c (λ x, g (f x)) :=
@@ -188,7 +179,6 @@ def simplify : Π (c : circuit α), circuit α
 | (or c₁ c₂) := simplify_or (simplify c₁) (simplify c₂)
 | (not c) := simplify_not (simplify c)
 | (xor c₁ c₂) := simplify_xor (simplify c₁) (simplify c₂)
-| (imp c₁ c₂) := simplify_imp (simplify c₁) (simplify c₂)
 
 @[simp] lemma eval_simplify : Π {c : circuit α} {f : α → bool},
   eval (simplify c) f = eval c f
@@ -199,7 +189,6 @@ def simplify : Π (c : circuit α), circuit α
 | (or c₁ c₂) f := by rw [simplify]; simp *
 | (not c) f := by rw [simplify]; simp *
 | (xor c₁ c₂) f := by rw [simplify]; simp *
-| (imp c₁ c₂) f := by rw [simplify]; simp *
 
 def sum_vars_left [decidable_eq α] [decidable_eq β] : circuit (α ⊕ β) → list α
 | true := []
@@ -210,7 +199,6 @@ def sum_vars_left [decidable_eq α] [decidable_eq β] : circuit (α ⊕ β) → 
 | (or c₁ c₂) := (sum_vars_left c₁ ++ sum_vars_left c₂).dedup
 | (not c) := sum_vars_left c
 | (xor c₁ c₂) := (sum_vars_left c₁ ++ sum_vars_left c₂).dedup
-| (imp c₁ c₂) := (sum_vars_left c₁ ++ sum_vars_left c₂).dedup
 
 def sum_vars_right [decidable_eq α] [decidable_eq β] : circuit (α ⊕ β) → list β
 | true := []
@@ -221,7 +209,6 @@ def sum_vars_right [decidable_eq α] [decidable_eq β] : circuit (α ⊕ β) →
 | (or c₁ c₂) := (sum_vars_right c₁ ++ sum_vars_right c₂).dedup
 | (not c) := sum_vars_right c
 | (xor c₁ c₂) := (sum_vars_right c₁ ++ sum_vars_right c₂).dedup
-| (imp c₁ c₂) := (sum_vars_right c₁ ++ sum_vars_right c₂).dedup
 
 lemma eval_eq_of_eq_on_vars [decidable_eq α] : Π {c : circuit α} {f g : α → bool}
   (h : ∀ x ∈ c.vars, f x = g x), eval c f = eval c g
@@ -248,13 +235,6 @@ begin
   rw [eval, eval, eval_eq_of_eq_on_vars h]
 end
 | (xor c₁ c₂) f g h :=
-begin
-  simp only [vars, list.mem_append, list.mem_dedup] at h,
-  rw [eval, eval,
-    eval_eq_of_eq_on_vars (λ x hx, h x (or.inl hx)),
-    eval_eq_of_eq_on_vars (λ x hx, h x (or.inr hx))]
-end
-| (imp c₁ c₂) f g h :=
 begin
   simp only [vars, list.mem_append, list.mem_dedup] at h,
   rw [eval, eval,
@@ -289,11 +269,6 @@ end
     simp [vars, sum_vars_left],
     simp [mem_vars_iff_mem_sum_vars_left]
   end
-| (imp c₁ c₂) _ :=
-  begin
-    simp [vars, sum_vars_left],
-    simp [mem_vars_iff_mem_sum_vars_left]
-  end
 
 @[simp] lemma mem_vars_iff_mem_sum_vars_right [decidable_eq α] [decidable_eq β] :
   Π {c : circuit (α ⊕ β)} {x : β},
@@ -318,11 +293,6 @@ end
     simp [mem_vars_iff_mem_sum_vars_right]
   end
 | (xor c₁ c₂) _ :=
-  begin
-    simp [vars, sum_vars_right],
-    simp [mem_vars_iff_mem_sum_vars_right]
-  end
-| (imp c₁ c₂) _ :=
   begin
     simp [vars, sum_vars_right],
     simp [mem_vars_iff_mem_sum_vars_right]
@@ -362,15 +332,6 @@ begin
   rw [eval, eval, eval_eq_of_eq_on_sum_vars_left_right h₁ h₂]
 end
 | (xor c₁ c₂) f g h₁ h₂ :=
-begin
-  simp only [sum_vars_left, sum_vars_right, list.mem_append, list.mem_dedup] at h₁ h₂,
-  rw [eval, eval,
-    eval_eq_of_eq_on_sum_vars_left_right
-      (λ x hx, h₁ x (or.inl hx)) (λ x hx, h₂ x (or.inl hx)),
-    eval_eq_of_eq_on_sum_vars_left_right
-      (λ x hx, h₁ x (or.inr hx)) (λ x hx, h₂ x (or.inr hx))]
-end
-| (imp c₁ c₂) f g h₁ h₂ :=
 begin
   simp only [sum_vars_left, sum_vars_right, list.mem_append, list.mem_dedup] at h₁ h₂,
   rw [eval, eval,
@@ -448,8 +409,6 @@ def assign_vars [decidable_eq α] :
 | (not c) f := simplify_not (assign_vars c (λ x hx, f x (by simp [hx, vars])))
 | (xor c₁ c₂) f := simplify_xor (assign_vars c₁ (λ x hx, f x (by simp [hx, vars])))
                         (assign_vars c₂ (λ x hx, f x (by simp [hx, vars])))
-| (imp c₁ c₂) f := simplify_imp (assign_vars c₁ (λ x hx, f x (by simp [hx, vars])))
-                        (assign_vars c₂ (λ x hx, f x (by simp [hx, vars])))
 
 lemma eval_assign_vars [decidable_eq α] : ∀ {c : circuit α}
   {f : Π (a : α) (ha : a ∈ c.vars), β ⊕ bool} {g : β → bool},
@@ -479,10 +438,6 @@ end
   simp [assign_vars, eval, vars],
   rw [eval_assign_vars, eval_assign_vars]
 end
-| (imp c₁ c₂) f g := begin
-  simp [assign_vars, eval, vars],
-  rw [eval_assign_vars, eval_assign_vars]
-end
 
 def bind : Π (c : circuit α) (f : α → circuit β), circuit β
 | true _ := true
@@ -492,7 +447,6 @@ def bind : Π (c : circuit α) (f : α → circuit β), circuit β
 | (or c₁ c₂) f := simplify_or (bind c₁ f) (bind c₂ f)
 | (not c) f := simplify_not (bind c f)
 | (xor c₁ c₂) f := simplify_xor (bind c₁ f) (bind c₂ f)
-| (imp c₁ c₂) f := simplify_imp (bind c₁ f) (bind c₂ f)
 
 lemma eval_bind : ∀ (c : circuit α) (f : α → circuit β) (g : β → bool),
   eval (bind c f) g = eval c (λ a, eval (f a) g)
@@ -512,10 +466,6 @@ end
   rw [eval_bind]
 end
 | (xor c₁ c₂) f g := begin
-  simp [bind, eval],
-  rw [eval_bind, eval_bind]
-end
-| (imp c₁ c₂) f g := begin
   simp [bind, eval],
   rw [eval_bind, eval_bind]
 end
@@ -539,5 +489,110 @@ begin
     cases x a ha; simp [h] }
 end
 
+def nonempty_aux [decidable_eq α] :
+  Π (c : circuit α), { b : bool // (∃ x, eval c x) = (b : Prop) }
+| true := ⟨tt, by simp⟩
+| false := ⟨ff, by simp⟩
+| (var x) := ⟨tt, by simp⟩
+-- | (or c₁ c₂) :=
+-- let b₁ := nonempty_aux c₁ in
+-- let b₂ := nonempty_aux c₂ in
+-- ⟨b₁ || b₂, by
+--   { simp only [exists_or_distrib, eval, bor_coe_iff, eq_iff_iff],
+--     rw [← b₁.prop, ← b₂.prop] }⟩
+-- | (and c₁ (or c₂ c₃)) :=
+-- let b₁ := nonempty_aux (and c₁ c₂) in
+-- let b₂ := nonempty_aux (and c₁ c₃) in
+-- ⟨b₁ || b₂, by
+--   { simp only [eval, bor_coe_iff, eq_iff_iff, band_coe_iff, and_or_distrib_left,
+--       exists_or_distrib],
+--     rw [← b₁.prop, ← b₂.prop],
+--     simp }⟩
+-- | (and (or c₁ c₂) c₃) :=
+-- let b₁ := nonempty_aux (and c₁ c₃) in
+-- let b₂ := nonempty_aux (and c₂ c₃) in
+-- ⟨b₁ || b₂, by
+--   { simp only [eval, bor_coe_iff, eq_iff_iff, band_coe_iff, or_and_distrib_right,
+--       exists_or_distrib],
+--     rw [← b₁.prop, ← b₂.prop],
+--     simp }⟩
+-- | (not (and c₁ c₂)) :=
+-- let b₁ := nonempty_aux (not c₁) in
+-- let b₂ := nonempty_aux (not c₂) in
+-- ⟨b₁ || b₂, by
+--   { simp only [eval, bor_coe_iff, eq_iff_iff, band_coe_iff, not_and_distrib, exists_or_distrib,
+--     bool.bnot_iff_not, eq_ff_eq_not_eq_tt],
+--     rw [← b₁.prop, ← b₂.prop],
+--     simp }⟩
+| c :=
+let v := vars c in
+have hv : vars c = v := rfl,
+match v, hv with
+| [], hv := ⟨eval c (λ _, ff), begin
+    rw [exists_eval_iff_exists_evalv, eq_iff_iff, eval_eq_evalv],
+    split,
+    { rintros ⟨x, hx⟩,
+      convert hx,
+      ext i hi,
+      rw [hv] at hi,
+      exact false.elim hi },
+    { intro h,
+      use λ i _, ff,
+      exact h }
+  end⟩
+| (i::l), hv :=
+let c₁ := c.assign_vars (λ j _, if i = j then sum.inr tt else sum.inl j) in
+let c₂ := c.assign_vars (λ j _, if i = j then sum.inr ff else sum.inl j) in
+have h₁ : sizeof c₁ < sizeof c := sorry,
+have h₂ : sizeof c₂ < sizeof c := sorry,
+let b₁ := nonempty_aux c₁ in
+let b₂ := nonempty_aux c₂ in
+⟨b₁ || b₂, begin
+  simp only [bor_coe_iff, eq_iff_iff, eval_eq_evalv],
+  rw [← b₁.prop, ← b₂.prop],
+  simp only [eval_assign_vars],
+  split,
+  { rintro ⟨x, hx⟩,
+    cases hi : x i,
+    { right,
+      use x,
+      convert hx,
+      ext j hj,
+      split_ifs,
+      { subst h,
+        simp [hi] },
+      { simp } },
+    { left,
+      use x,
+      convert hx,
+      ext j hj,
+      split_ifs,
+      { subst h,
+        simp [hi] },
+      { simp } } },
+  { intro h,
+    rcases h with ⟨x, hx⟩ | ⟨x, hx⟩,
+    { refine ⟨_, hx⟩ },
+    { refine ⟨_, hx⟩ } }
+end⟩
+end
+
+def nonempty [decidable_eq α] (c : circuit α) : bool :=
+(nonempty_aux c).1
+
+lemma nonempty_iff [decidable_eq α] (c : circuit α) :
+  nonempty c ↔ ∃ x, eval c x :=
+by rw [nonempty, ← (nonempty_aux c).2]
+
+def always_true [decidable_eq α] (c : circuit α) : bool :=
+bnot (nonempty (not c))
+
+lemma always_true_iff [decidable_eq α] (c : circuit α) :
+  always_true c ↔ ∀ x, eval c x :=
+by simp [always_true, nonempty_iff, not_not]
+
+instance [decidable_eq α] : decidable_rel ((≤) : circuit α → circuit α → Prop) :=
+λ c₁ c₂, decidable_of_iff (always_true ((not c₁).or c₂))
+  begin simp [always_true_iff, le_def, or_iff_not_imp_left], end
 
 end circuit
